pcuic/theories/PCUICToTemplate.v
@@ -11,11 +11,11 @@ Definition uint63_from_model (i : uint63_model) : Uint63.int :=
 Definition float64_from_model (f : float64_model) : PrimFloat.float :=
   FloatOps.SF2Prim (proj1_sig f).
     
-(* Definition trans_prim (t : prim_val) : Ast.term :=
+Definition trans_prim (t : prim_val) : Ast.term :=
   match t.π2 with
-  | primIntModel i => Ast.tInt (uint63_from_model i)
-  | primFloatModel f => Ast.tFloat (float64_from_model f)
-  end. *)
+  | primIntModel i => Ast.tInt i
+  | primFloatModel f => Ast.tFloat f
+  end.
 
 Definition trans_predicate (t : PCUICAst.predicate Ast.term) : predicate Ast.term :=
   {| pparams := t.(PCUICAst.pparams); 
@@ -51,7 +51,7 @@ Fixpoint trans (t : PCUICAst.term) : Ast.term :=
   | PCUICAst.tCoFix mfix idx =>
     let mfix' := List.map (map_def trans trans) mfix in
     tCoFix mfix' idx
-  (* | PCUICAst.tPrim i => trans_prim i *)
+  | PCUICAst.tPrim i => trans_prim i
   end.
 
 Notation trans_decl := (map_decl trans).
