template-coq/theories/Primitive.v
@@ -1,0 +1,18 @@
+(* Primitive types *)
+
+From Coq Require Import Int63 PrimFloat.
+From MetaCoq.Template Require Import bytestring MCString.
+Local Open Scope bs.
+
+Variant prim_tag := 
+  | primInt
+  | primFloat.
+  (* | primArray. *)
+Derive NoConfusion EqDec for prim_tag.
+
+Definition string_of_prim_int (i:Int63.int) : string := 
+  (* Better? DecimalString.NilZero.string_of_uint (BinNat.N.to_uint (BinInt.Z.to_N (Int63.to_Z i))). ? *)
+  string_of_Z (Numbers.Cyclic.Int63.Uint63.to_Z i).
+
+Definition string_of_float (f : PrimFloat.float) :=
+  "<float>".
